Finished proof of the always failing contract

example/AlwaysFail.thy
@@ -21,5 +21,62 @@ where
    , account_balance = balance
    , account_ongoing_calls = []
    \<rparr>"
+   
+definition always_fail_spec :: "uint \<Rightarrow> response_to_world"
+where
+" always_fail_spec initial_balance =
+  \<lparr> when_called = \<lambda> _. (ContractFail, always_fail_account_state initial_balance)
+  , when_returned = \<lambda> _. (ContractFail, always_fail_account_state initial_balance)
+  , when_failed = (ContractFail, always_fail_account_state initial_balance)
+  \<rparr>
+"
+
+inductive ev :: "nat \<Rightarrow> bool" where
+ev0: "ev 0" |
+evSS: "ev n \<Longrightarrow> ev (Suc (Suc n))"
+
+lemma "ev (Suc(Suc 0))"
+
+apply(rule evSS)
+apply (rule ev0)
+done
+
+lemma always_fail_correct:
+"
+  account_state_responds_to_world
+  (always_fail_account_state initial_balance)
+  (always_fail_spec initial_balance)
+  (\<lambda> _ _. True)
+"
+apply (simp add: always_fail_spec_def)
+apply (rule AccountStep)
+  apply(simp add: respond_to_call_correctly_def)
+  apply(rule allI)
+  apply(rule allI)
+  apply(rule impI)
+  apply(simp add: always_fail_account_state_def)
+  apply(simp add: always_fail_code_def)
+  apply(simp add: build_cenv_def)
+  apply(simp add: build_venv_called.simps)
+  apply(auto)
+  apply(case_tac steps)
+   apply(auto)
+  apply(simp add: stack_0_1_op_def add: venv_advance_pc_def add: drop_one_element_def)
+  apply(case_tac nat)
+   apply(auto)
+  apply(simp add: jump_def add: venv_stack_top_def add: venv_change_sfx_def
+             add: venv_first_instruction_def add: word_rcat_def)
+  apply(simp add: unat_def)
+  apply(simp add: bin_rcat_def)
+  apply(simp add: instruction_failure_result_def)
+  apply(simp add: update_account_state_def)
+ apply(simp add: respond_to_return_correctly_def)
+ apply(simp add: always_fail_account_state_def)
+ apply(simp add: build_cenv_def)
+ apply(simp add: build_venv_returned.simps)
+apply(simp add: respond_to_fail_correctly_def)
+apply(simp add: build_venv_fail_def)
+apply(simp add: always_fail_account_state_def)
+done
 
 end
